.

ImportGraph/Tools/FindHome.lean
@@ -13,6 +13,7 @@ public meta import ImportGraph.Graph.TransitiveClosure
 meta import all Lean.ExtraModUses
 public meta import Lake.CLI.Shake
 import all Lake.CLI.Shake
+import all Lean.Elab.Command
 
 open Lean Lake Shake
 
@@ -26,7 +27,29 @@ We have some functionality we need.
 - minimize: full import set → minimal direct imports
 - import set → meet
 
+
+thinking a bit: we could track not only which imports are needed, but why. Which declarations are needed from those modules? This is harder.
+
 -/
+
+meta section
+
+/--
+This declaration exists in `Batteries`, but we don't want to make `ImportGraph` depend on batteries. We therefore just bear the duplication cost and make this private (and primed, in case someone `imports all`).
+-/
+private protected def Lean.Position.getDeclsAfter' (env : Environment) (pos : Position)
+    (asyncMode := EnvExtension.AsyncMode.local) : Array Name :=
+  declRangeExt.getState env asyncMode |>.foldl (init := #[])
+    fun acc name { selectionRange .. } =>
+      if selectionRange.pos.lt pos then acc else acc.push name
+
+/--
+Likewise
+-/
+@[inline] private protected def _root_.String.Pos.Raw.getDeclsAfter' (env : Environment) (map : FileMap)
+    (pos : String.Pos.Raw) (asyncMode := EnvExtension.AsyncMode.local) : Array Name :=
+  map.toPosition pos |>.getDeclsAfter' env asyncMode
+
 
 /-- Debugging: list every `(j, k)` entry in `needs` as a literal `Import`, with no deduplication
 across kinds. `modNames` maps `ModuleIdx` to `Name` (e.g. `State.modNames`). -/
@@ -89,29 +112,32 @@ deriving instance Ord for NeedsKind
 /-- A set of `NeedsKind`s. -/
 abbrev NeedsKindSet := Std.TreeSet NeedsKind
 
-/-- States that the (local) declarations `foo` are needed at their assigned sets of `NeedsKind`s. For instance, if `foo` is used in an exporting position, such as a public def's type, it will acquire `foo ↦ {{ isExported := true, isMeta := false }}`. -/
--- We might be able to simplify this to not be a set.
-abbrev DeclNeeds := NameMap NeedsKindSet
+/-- Assigns `bar` to the (local) declarations `foo` that are needed at their assigned sets of `NeedsKind`s. For instance, if `foo` is used in an exporting position, such as a public def's type, it will acquire `foo ↦ {{ isExported := true, isMeta := false }}`. -/
+-- We might be able to simplify this quite a bit.
+abbrev DeclNeeds := NameMap (NameMap NeedsKindSet)
 
-nonrec def DeclNeeds.insert (k : NeedsKind) (decl : Name) (needs : DeclNeeds) :=
+nonrec def DeclNeeds.insert (k : NeedsKind) (decl usedDecl : Name) (needs : DeclNeeds) :=
   needs.alter decl fun
-    | none => some {k}
-    | some ks => ks.insert k
+    | none => some (.empty |>.insert usedDecl {k})
+    | some usedDecls => some <| usedDecls.alter usedDecl fun
+      | none => some {k}
+      | some ks => ks.insert k
 
 /--
-Calculates the needs for a given module `mod` from constants and recorded extra uses.
+Calculates the needs for a given module `mod` from constants and recorded extra uses. Note that this does not calculate transitive needs, and assumes we're running from within the same file as the declaration.
 
 Does not account for `extraModUses`, since these are not decl-linked per se.
 
-Collects needed declarations from the current module in `DeclNeeds`, together with the visibiility they're needed at.
+Collects needed declarations from the current module in `DeclNeeds`, together with the visibiility they're needed at. Includes the needs of those declarations (not accounting for elaborator needs in their respective commands).
 -/
-def calcDeclNeeds? (decl : Name) (env : Environment)
-    (needs : Needs := .empty) (extraDecls : DeclNeeds := {}) : Option (Needs × DeclNeeds) :=
+-- Largely copied from `calcNeeds`, but with some key differences.
+partial def calcDeclNeeds (decl : Name) (env : Environment)
+    (needs : Needs := .empty) (extraDecls : DeclNeeds := {}) : Needs × DeclNeeds :=
   Id.run do
   let mut needs := needs
   let mut extraDecls := extraDecls
   let indirectModUses := indirectModUseExt.getState env
-  let some ci := env.find? decl | return none
+  let some ci := env.find? decl | return default
   -- Added guard for cases like `structure` that are still exported even if private
   let pubCI? := guard (!isPrivateName ci.name) *> (env.setExporting true).find? ci.name
   let k := { isExported := pubCI?.isSome, isMeta := isDeclMeta' env ci.name }
@@ -121,12 +147,11 @@ def calcDeclNeeds? (decl : Name) (env : Environment)
     let k := if k.isMeta then k else
       if pubCI?.any (·.hasValue (allowOpaque := true)) then .pub else .priv
     (needs, extraDecls) := visitExpr indirectModUses k e needs extraDecls
-
   return (needs, extraDecls)
 where
   /-- Accumulate the results from expression `e` into `deps`. -/
   visitExpr (indirectModUses : Std.HashMap Name (Array ModuleIdx)) (k : NeedsKind) (e : Expr)
-      (deps : Needs) (extras : DeclNeeds) : (Needs × DeclNeeds) :=
+      (deps : Needs) (extras : DeclNeeds) : Needs × DeclNeeds :=
     Lean.Expr.foldConsts e (deps, extras) fun c (deps, extras) => Id.run do
       let mut deps := deps
       let mut extras := extras
@@ -140,11 +165,364 @@ where
               deps := deps.union k {indMod}
         else
           -- `c` is from the same module--we need it at the given `k`
-          extras := extras.insert k c
+          unless extras.contains c || c == decl do -- just in case
+            extras := extras.insert k decl c
+            (deps, extras) := calcDeclNeeds c env deps extras
       return (deps, extras)
 
-def
+meta instance : ToMessageData ExtraModUse where
+  toMessageData a := m!"⟦{if a.isExported then "public " else ""}{if a.isMeta then "meta " else ""}{a.module.toString}⟧"
 
+meta instance : ToMessageData IndirectModUse where
+  toMessageData a := m!"⟦{a.kind}{.ofConstName a.declName}⟧"
+
+meta def Std.HashMap.subtractArray {α} {β} [BEq α] [BEq β] [Hashable α]
+    (s₁ s₂ : Std.HashMap α (Array β)) (deleteEmpty := true) : Std.HashMap α (Array β) := Id.run do
+  let mut s := s₁
+  for (key, vals₂) in s₂ do
+    s := s.alter key fun
+      | none => none
+      | some vals =>
+        let vals := vals.filter (!vals₂.contains ·)
+        if vals.isEmpty && deleteEmpty then none else vals
+  return s
+
+open Elab Command in
+elab "#show_shake" ppLine cmd:command : command => do
+  let env ← getEnv
+  let initExtraModUses := PersistentEnvExtension.getState extraModUses env
+  let initIndirectModUses := PersistentEnvExtension.getState indirectModUseExt env
+  let initIsRev := !(isExtraRevModUseExt.getEntries env |>.isEmpty)
+  elabCommandTopLevel cmd
+  recordUsedSyntaxKinds cmd
+  let env ← getEnv
+
+  let extraModUses := PersistentEnvExtension.getState extraModUses env .sync
+  let indirectModUses := PersistentEnvExtension.getState indirectModUseExt env
+  let isRev := !(isExtraRevModUseExt.getEntries env |>.isEmpty)
+  logInfo m!"extraModUses:\n  \
+    {extraModUses.1.filter (!initExtraModUses.1.contains ·)}\n  \
+    {extraModUses.2.toList.filter (!initExtraModUses.2.contains ·)}\n\
+  indirectModUses:\n  \
+    {indirectModUses.1.filter (!initIndirectModUses.1.contains ·)}\n  \
+    {indirectModUses.2.subtractArray initIndirectModUses.2 |>.toList}\n\
+  isNewRev: {isRev && !initIsRev}"
+
+/-
+Notes:
+
+- Macros and tactic elaborators automatically record extraModUses.
+- Term and command elaborators do not.
+- `elabCommandTopLevel` runs the private def `recordUsedSyntaxKinds` which records an extra mod use for every syntax kind.
+  - Usually, this suffices to cover the modules of term and command elaborators, which are usually defined in the same module as the syntax.
+  - Ones that aren't should record the extra module use manually.
+
+
+-/
+
+-- set_option Elab.async false
+#show_shake
+def foo : MetaM Bool := do
+  let stx ← `(term| NameMap.transitiveClosure)
+  return test2%
+
+
+#check indirectModUseExt
+#show_shake
+macro "aa" : command => `(command|#check true)
+
+meta section
+
+def Lean.SimplePersistentEnvExtension.modifyEntries (env : Environment)
+    (ext : SimplePersistentEnvExtension α σ) (f : List α → List α)
+    (asyncMode : EnvExtension.AsyncMode := ext.toEnvExtension.asyncMode)
+    (asyncDecl : Name := Name.anonymous) : Environment :=
+  PersistentEnvExtension.modifyState ext env (fun (entries, s) => (f entries, s))
+    asyncMode asyncDecl
+
+def Lean.SimplePersistentEnvExtension.setEntries (env : Environment)
+    (ext : SimplePersistentEnvExtension α σ) (entries : List α)
+    (asyncMode : EnvExtension.AsyncMode := ext.toEnvExtension.asyncMode)
+    (asyncDecl : Name := Name.anonymous) : Environment :=
+  PersistentEnvExtension.modifyState ext env (fun (_, s) => (entries, s))
+    asyncMode asyncDecl
+
+
+/-- Resets the state of the `indirectModUse` extension. Note that the state is never altered in the course of the file, as it only represents imported entries. Only the entries list is gotten/reset. -/
+@[inline] def resetIndirectModUses (env : Environment)
+    (asyncMode : EnvExtension.AsyncMode := indirectModUseExt.toEnvExtension.asyncMode)
+    (asyncDecl : Name := Name.anonymous) :
+    Environment :=
+  indirectModUseExt.setEntries env [] asyncMode asyncDecl
+
+@[inline] def getIndirectModUsesState (env : Environment)
+    (asyncMode : EnvExtension.AsyncMode := indirectModUseExt.toEnvExtension.asyncMode) :
+    List IndirectModUse :=
+  indirectModUseExt.getEntries env asyncMode
+
+@[inline] def setIndirectModUsesState (env : Environment) (entries : List IndirectModUse)
+    (asyncMode : EnvExtension.AsyncMode := indirectModUseExt.toEnvExtension.asyncMode)
+    (asyncDecl : Name := Name.anonymous) :
+    Environment :=
+  indirectModUseExt.setEntries env entries asyncMode asyncDecl
+
+/-- Gets and resets the state of the `indirectModUse` extension. Note that the state is never altered in the course of the file, as it only represents imported entries. Only the entries list is gotten/reset. -/
+def getResetIndirectModUses (env : Environment)
+    (asyncMode : EnvExtension.AsyncMode := indirectModUseExt.toEnvExtension.asyncMode)
+    (asyncDecl : Name := Name.anonymous) :
+    List IndirectModUse × Environment :=
+  letI indirect := indirectModUseExt.getEntries env asyncMode
+  (indirect, resetIndirectModUses env asyncMode asyncDecl)
+
+@[inline] def resetExtraModUses (env : Environment) :
+    Environment :=
+  PersistentEnvExtension.setState extraModUses env ([], {})
+
+@[inline] def getExtraModUsesState (env : Environment)
+    (asyncMode : EnvExtension.AsyncMode := extraModUses.toEnvExtension.asyncMode)
+    (asyncDecl : Name := Name.anonymous) :
+    List ExtraModUse × PHashSet ExtraModUse :=
+  PersistentEnvExtension.getState extraModUses env asyncMode asyncDecl
+
+@[inline] def setExtraModUsesState (env : Environment)
+    (entries : List ExtraModUse)
+    (state : PHashSet ExtraModUse) :
+    Environment :=
+  PersistentEnvExtension.setState extraModUses env (entries, state)
+
+
+/-- Gets and resets the state of the `extraModUses` extension. Note that the state does not include imported entries. -/
+def getResetExtraModUses (env : Environment)
+    (asyncMode : EnvExtension.AsyncMode := extraModUses.toEnvExtension.asyncMode)
+    (asyncDecl : Name := Name.anonymous) :
+    (List ExtraModUse × PHashSet ExtraModUse) × Environment :=
+  (getExtraModUsesState env asyncMode asyncDecl, resetExtraModUses env)
+
+
+/-- Gets the state of the `extraModUses` extension. -/
+@[inline] def getIsExtraRevModUse (env : Environment) : Bool :=
+  !(isExtraRevModUseExt.getEntries env |>.isEmpty)
+
+/-- Resets the state of the `extraModUses` extension. -/
+@[inline] def resetIsExtraRevModUse (env : Environment)
+    (asyncMode : EnvExtension.AsyncMode := isExtraRevModUseExt.toEnvExtension.asyncMode)
+    (asyncDecl : Name := Name.anonymous) :
+    Environment :=
+  if getIsExtraRevModUse env then
+    isExtraRevModUseExt.setEntries env [] asyncMode asyncDecl else env
+
+/-- Resets the state of the `extraModUses` extension. -/
+@[inline] def setIsExtraRevModUse (env : Environment) (isRev : Bool)
+    (asyncMode : EnvExtension.AsyncMode := isExtraRevModUseExt.toEnvExtension.asyncMode)
+    (asyncDecl : Name := Name.anonymous) :
+    Environment :=
+  if getIsExtraRevModUse env == isRev then env else
+    isExtraRevModUseExt.setEntries env (if isRev then [()] else []) asyncMode asyncDecl
+
+/-- Merges the state of the `extraModUses` extension (using "or" semantics). -/
+@[inline] def mergeIsExtraRevModUse (env : Environment) (old : Bool)
+    (asyncMode : EnvExtension.AsyncMode := isExtraRevModUseExt.toEnvExtension.asyncMode)
+    (asyncDecl : Name := Name.anonymous) :
+    Environment :=
+  if old then setIsExtraRevModUse env old asyncMode asyncDecl else env
+
+/-- Gets and resets the state of the `extraModUses` extension. -/
+def getResetIsExtraRevModUse (env : Environment)
+    (asyncMode : EnvExtension.AsyncMode := isExtraRevModUseExt.toEnvExtension.asyncMode)
+    (asyncDecl : Name := Name.anonymous) :
+    Bool × Environment :=
+  if isExtraRevModUseExt.getEntries env |>.isEmpty then
+    (false, env)
+  else
+    (true, isExtraRevModUseExt.setEntries env [] asyncMode asyncDecl)
+
+def resetShakeExts (env : Environment) (asyncMode : EnvExtension.AsyncMode := .sync)
+    (asyncDecl : Name := Name.anonymous) : Environment :=
+  letI env := resetIndirectModUses env asyncMode asyncDecl
+  letI env := resetExtraModUses env
+  resetIsExtraRevModUse env asyncMode asyncDecl
+
+def List.prependWithoutDuplicating [BEq α] (as bs : List α) : List α :=
+  match as with
+  | [] => bs
+  | a :: as => let new := as.prependWithoutDuplicating bs; if new.contains a then new else a :: new
+
+def Lean.PHashSet.union {α} [BEq α] [Hashable α] (as bs : PHashSet α) : PHashSet α := Id.run do
+  let mut bs := bs
+  for a in as do
+    unless bs.contains a do
+      bs := bs.insert a
+  return bs
+
+-- TODO: could take an approach more like `copyExtraModUses`, possibly even use it. But we don't need to retain the whole environment...
+/-- Resets the shake extensions that record modules, then restores them after running the given action, merging any new records into the new ones. -/
+def withFreshModRecords [Monad m] [MonadEnv m] [MonadFinally m] {α} (x : m α)
+    (asyncMode : EnvExtension.AsyncMode := .sync)
+    (asyncDecl : Name := Name.anonymous) : m α := do
+  let indirect := getIndirectModUsesState (← getEnv) asyncMode
+  let (extraEntries, extraState) := getExtraModUsesState (← getEnv) asyncMode asyncDecl
+  let isRev := getIsExtraRevModUse (← getEnv)
+  modifyEnv (resetShakeExts · asyncMode asyncDecl)
+  try
+    x
+  finally
+    modifyEnv fun env =>
+      letI newIndirect := getIndirectModUsesState env asyncMode
+      letI env := setIndirectModUsesState env (newIndirect.prependWithoutDuplicating indirect) asyncMode asyncDecl
+      let (newExtraEntries, newExtraState) := getExtraModUsesState env asyncMode asyncDecl
+      letI env := setExtraModUsesState env
+        (newExtraEntries.prependWithoutDuplicating extraEntries)
+        (newExtraState.union extraState)
+      mergeIsExtraRevModUse env isRev asyncMode asyncDecl
+
+open Elab Command in
+elab "#show_imports" ppLine cmd:command : command => do
+  let needs ← withFreshModRecords do
+    elabCommand cmd
+    recordUsedSyntaxKinds cmd
+    let indirect := getIndirectModUsesState (← getEnv)
+    let (extras, _) := getExtraModUsesState (← getEnv)
+    let decls := cmd.raw.getPos?.get!.getDeclsAfter' (← getEnv) (← getFileMap)
+    let mut needs := .empty
+    let mut declNeeds := {}
+    for decl in decls do
+      (needs, declNeeds) := calcDeclNeeds decl (← getEnv) needs declNeeds
+    pure (needs, declNeeds, indirect, extras)
+  logInfo m!"{needs.1.toMessageData (← getEnv)}{needs.2.2}"
+
+/-
+#min_imports as widget that waits for everything by adding a linter that holds a handle to a promise, which is resolved in the infoview? Is that possible?
+
+Also something that just minimizes your existing imports into something canonical.
+
+Should respect shake directives.
+-/
+
+/-- Written mostly by claude. -/
+@[specialize f]
+def Lake.Shake.Bitset.foldOneIdxs (s : Bitset) (init : α) (f : α → Nat → α) : α := Id.run do
+  let mut n := s.toNat
+  let mut acc := init
+  while n != 0 do
+    let i := n.log2  -- highest bit, O(1) on GMP
+    acc := f acc i   -- (visits high→low; flip if you need low→high)
+    n := n ^^^ (1 <<< i)
+  return acc
+
+/-- High to low. -/
+def Lake.Shake.Bitset.toIdxs (s : Bitset) : Array Nat := s.foldOneIdxs #[] (·.push ·)
+
+instance {m} [Monad m] : ForIn m Bitset Nat where
+  forIn s init f := do
+    let mut n := s.toNat
+    let mut acc := init
+    while n != 0 do
+      let i := n.log2
+      match ← f i acc with
+      | .done b => return b
+      | .yield b => acc := b
+      n := n ^^^ (1 <<< i)
+    return acc
+
+instance {m} [Monad m] : ForIn m Needs (NeedsKind × Nat) where
+  forIn s init f := do
+    let mut acc := init
+    for k in NeedsKind.all do
+      let mut n := s.get k |>.toNat
+      while n != 0 do
+        let i := n.log2
+        match ← f (k, i) acc with
+        | .done b => return b
+        | .yield b => acc := b
+        n := n ^^^ (1 <<< i)
+    return acc
+
+namespace Lake.Shake
+/-
+`#find_home` now just needs
+- turn `Needs` into surface imports (easy)
+- meet operation on `Needs`. Might need transitive deps after all.
+-/
+
+/-- Reflexively transitively closes a `Needs`. -/
+def Needs.transitiveClosure (directNeeds : Needs) (transDeps : Array Needs) : Needs := Id.run do
+  let mut needs := directNeeds
+  for (k, i) in directNeeds do
+    needs := addTransitiveImps needs { k with module := .anonymous } i transDeps[i]!
+  return needs
+  -- or:
+  -- let mut needs := directNeeds
+  -- for h : i in 0...transDeps.size do
+  --   for k in NeedsKind.all do
+  --     if directNeeds.has k i then
+  --       needs := addTransitiveImps needs { k with module := .anonymous } i transDeps[i]
+  -- return needs
+
+@[inline] def Bitset.le (a b : Bitset) : Bool := a.toNat &&& b.toNat == a.toNat
+@[inline] def Bitset.intersect (a b : Bitset) : Bitset where
+  toNat := a.toNat &&& b.toNat
+
+/-- Assumes the second argument is already transitively closed (not necessarily the first), and also has b.pub ≤ b.priv. Does not transitively close the `Needs`. `false` includes incomparable. -/
+@[inline] def Needs.le (a b : Needs) : Bool :=
+  -- NeedsKind.all.all fun k => a.get k |>.le b.get k
+  a.pub.le b.pub
+    && a.priv.le b.priv
+    && a.metaPub.le b.metaPub
+    && a.metaPriv.le b.metaPriv
+
+theorem le_eq_all_get_le_get (a b : Needs) :
+    a.le b = NeedsKind.all.all fun k => a.get k |>.le <| b.get k := by
+  simp [NeedsKind.all, Needs.get, Needs.le, Bool.and_assoc]
+
+def Needs.fillPriv (a : Needs) : Needs :=
+  { a with priv := a.priv ∪ a.pub, metaPriv := a.metaPriv ∪ a.metaPub }
+
+/-- Assumes the second argument is already transitively closed (not necessarily the first). Does not transitively close the `Needs`. `false` includes incomparable. -/
+def Needs.le' (a b : Needs) : Bool :=
+  a.pub.le b.pub
+    && a.metaPub.le b.metaPub
+    && a.priv.le (b.priv ∪ b.pub)
+    && a.metaPriv.le (b.metaPriv ∪ b.metaPub)
+
+@[inline] def Needs.reflexify (i : Nat) (a : Needs) : Needs where
+  pub := a.pub ∪ {i}
+  priv := a.priv ∪ {i}
+  metaPub := a.metaPub ∪ {i}
+  metaPriv := a.metaPriv ∪ {i}
+
+def Needs.fillTransDeps (transDeps : Array Needs) : Array Needs :=
+  transDeps.mapIdx fun i n => n.fillPriv.reflexify i
+
+@[inline] def _root_.Array.filter' (a : Array α) (f : α → Bool) : Array α × Bool :=
+  let s := a.size
+  let a := a.filter f
+  (a, a.size ≠ s)
+
+@[inline] def _root_.Array.incorporateBelow (as : Array (Option α)) (a : α)
+    (le : α → α → Bool) : Array (Option α) := Id.run do
+  let mut as := as
+  for i in 0...as.size do
+    let some aᵢ := as[i]! | continue
+    if le a aᵢ then
+      as := as.set! i none
+    else if le aᵢ a then
+      return as
+  return as.push a
+
+
+/-- `needs` does not need to be transitively closed. -/
+def Needs.coverings (filledRflTransDeps : Array Needs) (needs : Needs) : Array ModuleIdx := Id.run do
+  let mut mods := #[]
+  let mut b := false
+  for h : i in 0...filledRflTransDeps.size do
+    if needs.le filledRflTransDeps[i] then
+      mods := mods.incorporateBelow i fun a b => filledRflTransDeps[a]!.le filledRflTransDeps[b]!
+  return mods.reduceOption
+
+
+
+
+#show_imports
 /--
 Find locations as high as possible in the import hierarchy
 where the named declaration could live.
@@ -180,6 +558,8 @@ meta def fooLinter : Linter where
     -- let r := isExtraRevModUseExt.getState (← getEnv)
 
 -- #check record
+
+#check initStateFromEnv
 
 run_cmd do
   lintersRef.modify fun ls => ls.filter (·.name != `foo)
